Weidenbach_Book/CDCL_Two_Watched_Literals_Watch_List_Domain.thy
@@ -212,6 +212,9 @@ text \<open>This is the \<^emph>\<open>completion\<close> of \<^term>\<open>\<A>
   literal of \<^term>\<open>\<A>\<^sub>i\<^sub>n\<close>:\<close>
 definition \<L>\<^sub>a\<^sub>l\<^sub>l where \<open>\<L>\<^sub>a\<^sub>l\<^sub>l = poss \<A>\<^sub>i\<^sub>n + negs \<A>\<^sub>i\<^sub>n\<close>
 
+lemma atms_of_\<L>\<^sub>a\<^sub>l\<^sub>l_\<A>\<^sub>i\<^sub>n: \<open>atms_of \<L>\<^sub>a\<^sub>l\<^sub>l = set_mset \<A>\<^sub>i\<^sub>n\<close>
+  unfolding \<L>\<^sub>a\<^sub>l\<^sub>l_def by (auto simp: atms_of_def image_Un image_image)
+
 definition is_\<L>\<^sub>a\<^sub>l\<^sub>l :: "nat literal multiset \<Rightarrow> bool" where
   \<open>is_\<L>\<^sub>a\<^sub>l\<^sub>l S \<longleftrightarrow> set_mset S = set_mset \<L>\<^sub>a\<^sub>l\<^sub>l\<close>
 
@@ -288,13 +291,25 @@ lemma literals_are_in_\<L>\<^sub>i\<^sub>n_mm_in_\<L>\<^sub>a\<^sub>l\<^sub>l:
 proof -
   have \<open>xs ! i \<in># mset xs\<close>
     using i_xs by auto
-  thm in_all_lits_of_m_ain_atms_of_iff
   then have \<open>xs ! i ! j \<in> set_mset (all_lits_of_mm (mset `# mset xs))\<close>
     using j_xs by (auto simp: in_all_lits_of_mm_ain_atms_of_iff atms_of_ms_def Bex_def
       intro!: exI[of _ \<open>xs ! i\<close>])
   then show ?thesis
     using N1 unfolding literals_are_in_\<L>\<^sub>i\<^sub>n_mm_def by blast
 qed
+
+definition literals_are_in_\<L>\<^sub>i\<^sub>n_trail :: \<open>(nat, 'mark) ann_lits \<Rightarrow> bool\<close> where
+  \<open>literals_are_in_\<L>\<^sub>i\<^sub>n_trail M \<longleftrightarrow> set_mset (lit_of `# mset M) \<subseteq> set_mset \<L>\<^sub>a\<^sub>l\<^sub>l\<close>
+
+lemma literals_are_in_\<L>\<^sub>i\<^sub>n_trail_in_lits_of_l:
+  \<open>literals_are_in_\<L>\<^sub>i\<^sub>n_trail M \<Longrightarrow> a \<in> lits_of_l M \<Longrightarrow> a \<in># \<L>\<^sub>a\<^sub>l\<^sub>l\<close>
+  by (auto simp: literals_are_in_\<L>\<^sub>i\<^sub>n_trail_def lits_of_def)
+
+lemma literals_are_in_\<L>\<^sub>i\<^sub>n_trail_in_lits_of_l_atms:
+  \<open>literals_are_in_\<L>\<^sub>i\<^sub>n_trail M \<Longrightarrow> a \<in> lits_of_l M \<Longrightarrow> atm_of a \<in># \<A>\<^sub>i\<^sub>n\<close>
+  using literals_are_in_\<L>\<^sub>i\<^sub>n_trail_in_lits_of_l[of M a]
+  unfolding in_\<L>\<^sub>a\<^sub>l\<^sub>l_atm_of_in_atms_of_iff[symmetric] atms_of_\<L>\<^sub>a\<^sub>l\<^sub>l_\<A>\<^sub>i\<^sub>n[symmetric]
+  .
 
 abbreviation D\<^sub>0 :: \<open>(nat \<times> nat literal) set\<close> where
   \<open>D\<^sub>0 \<equiv> (\<lambda>L. (nat_of_lit L, L)) ` set_mset \<L>\<^sub>a\<^sub>l\<^sub>l\<close>
@@ -394,9 +409,6 @@ proof -
   show ?thesis
     using H unfolding 1 2 3 .
 qed
-
-lemma atms_of_\<L>\<^sub>a\<^sub>l\<^sub>l_\<A>\<^sub>i\<^sub>n: \<open>atms_of \<L>\<^sub>a\<^sub>l\<^sub>l = set_mset \<A>\<^sub>i\<^sub>n\<close>
-  unfolding \<L>\<^sub>a\<^sub>l\<^sub>l_def by (auto simp: atms_of_def image_Un image_image)
 
 lemma literals_are_in_\<L>\<^sub>i\<^sub>n_in_\<L>\<^sub>a\<^sub>l\<^sub>l:
   assumes
